latest boogie files

DoubleCount.java
@@ -1,0 +1,10 @@
+class DoubleCount {
+int val;
+int dbl;
+
+}
+
+public static void main(String[] args)
+{
+
+}
