composite1.bpl
@@ -33,68 +33,64 @@ axiom (forall this: Ref, left: [Ref]Ref, right: [Ref]Ref, parent:[Ref]Ref::
     (this!=null) && (parent[this]!=null) ==>((this==right[parent[this]]) || (this==left[parent[this]]))
 );
 
-procedure PackLeft(this:Ref, lc:int);
-ensures ((  (left[this] != null) && 
+procedure PackLeftNotNull(this:Ref, lc:int);
+requires (left[this] != null) && 
        packed[left[this], countP] &&
        (cCountPred[left[this]] == lc) &&
-       (frac[left[this], countP] >= 50) ) 
-                      ==> ( packed[this, leftP] && (lcLeftPred[this] == lc) ) )
-  &&
-  ( ( (left[this] == null) && (lc==0) ) ==> ( packed[this, leftP] && (lcLeftPred[this] == 0) ) );
+       (frac[left[this], countP] >= 50);  
+ensures (lcLeftPred[this] == lc);
+
+
+procedure PackLeftNull(this:Ref, lc:int);
+requires (left[this] == null) && (lc==0);
+ensures (lcLeftPred[this] == 0);
 
 procedure UnpackLeftNull(this:Ref, lc:int);
-ensures (packed[this, leftP] && (lcLeftPred[this] == 0) ==> (left[this] == null) );
+requires packed[this, leftP] && (lcLeftPred[this] == 0);
+ensures left[this] == null;
 
 procedure UnpackLeftNotNull(this:Ref, lc:int);
-ensures ( (packed[this, leftP] && (lcLeftPred[this] == lc) && (left[this] != null) )
-   ==> 
-  (  packed[left[this], countP] &&
+requires packed[this, leftP] && (lcLeftPred[this] == lc) && (left[this] != null);
+ensures  packed[left[this], countP] &&
        (cCountPred[left[this]] == lc)
-     && (frac[left[this], countP] >= 50) ) );
+     && (frac[left[this], countP] >= 50);
 
 
-procedure PackRight(this:Ref, rc:int);
-ensures  ((  (right[this] != null) && 
+procedure PackRightNotNull(this:Ref, rc:int);
+requires  (right[this] != null) && 
    packed[right[this], countP] &&
    (cCountPred[right[this]] == rc) &&
- (frac[right[this], countP] >= 50) ) 
-                       ==> 
-(packed[this, rightP] && (rcRightPred[this] == rc)))
-  &&
-  ((  (right[this] == null) && (rc==0) ) ==> 
-packed[this, rightP] && (rcRightPred[this] == 0)
-);
+ (frac[right[this], countP] >= 50) ;
+ensures (rcRightPred[this] == rc);
+
+procedure PackRightNull(this:Ref, rc:int);
+requires   (right[this] == null) && (rc==0);
+ensures (rcRightPred[this] == 0);
 
 procedure UnpackRightNull(this:Ref, rc:int);
-ensures (packed[this, rightP] && (rcRightPred[this] == 0) ==> (right[this] == null) );
+requires packed[this, rightP] && (rcRightPred[this] == 0);
+ensures right[this] == null;
 
 procedure UnpackRightNotNull(this:Ref, rc:int);
-ensures (packed[this, rightP] && (rcRightPred[this] == rc) && (right[this] != null) ==> 
- ( packed[right[this], countP] && (cCountPred[right[this]] == rc) && (frac[right[this], countP] >= 50) ));
+requires packed[this, rightP] && (rcRightPred[this] == rc) && (right[this] != null);
+ensures  packed[right[this], countP] &&
+ (cCountPred[right[this]] == rc) && (frac[right[this], countP] >= 50);
 
 procedure PackCount(this:Ref, c:int);
-ensures  ( ( (this!=null) && (
-  exists lc: int, rc:int ::
-  ( packed[this, leftP] && (lcLeftPred[this] == lc) && 
-  (frac[this, leftP] >= 50) &&
-  packed[this, rightP] &&
-  (rcRightPred[this] == rc) &&
-(frac[this, rightP] >= 50) && 
- (count[this] == lc+rc+1) &&
- ( count[this]== c) )
-) ) ==> 
-packed[this, countP] &&
-(cCountPred[this] == c)
+requires  (this!=null) && (
+  ( exists lc: int, rc:int ::
+   countPredFunc(this, count,  lc, rc, 
+        lcLeftPred, rcRightPred, packed, frac) ) &&
+ ( count[this]== c)
 );
+ensures (cCountPred[this] == c);
 
 procedure UnpackCount(this:Ref, c:int);
-ensures ( (packed[this, countP] && 
-  cCountPred[this] == c
-) ==>
-    ( (this!=null) && (
+requires packed[this, countP] && 
+  cCountPred[this] == c;
+ensures    (this!=null) && (
   exists lc: int, rc:int ::
-  (
-packed[this, leftP] &&
+  (packed[this, leftP] &&
 (lcLeftPred[this] == lc) &&
  (frac[this, leftP] >= 50) &&
  packed[this, rightP] &&
@@ -102,7 +98,7 @@ packed[this, leftP] &&
  (frac[this, rightP] >= 50) && 
  (count[this] == lc+rc+1) &&
  ( count[this]== c) )
-) ) );
+);
 
 
 
@@ -110,8 +106,7 @@ packed[this, leftP] &&
 axiom (forall this:Ref,count: [Ref]int :: (this==null) ==> (count[this]==0)  );
 
 procedure PackParentNotNull(this:Ref);
-ensures   (
-    (parent[this] != this) &&
+requires   (parent[this] != this) &&
     packed[this, countP] &&
     (cCountPred[this] == count[this]) &&
      (frac[this, countP]>=50) &&
@@ -125,24 +120,18 @@ ensures   (
            ( packed[parent[this], rightP] &&
              rcRightPred[parent[this]] ==count[this] &&
             (frac[parent[this], rightP] >= 50))
-           ))  
-  ==>
-  packed[this, parentP];
+           );
 
 procedure PackParentNull(this:Ref);
-ensures (
-  (parent[this] != this) &&
+requires (parent[this] != this) &&
    packed[this, countP] &&
    cCountPred[this] == count[this] &&
    (frac[this, countP]>=100) &&
-   (parent[this]==null)
-  )
-  ==>
-    packed[this, parentP];
+   (parent[this]==null);
 
 procedure UnpackParent(this:Ref);
-ensures ( packed[this, parentP] ==>
-  ( (parent[this] != this)
+requires packed[this, parentP];
+ensures (parent[this] != this)
        &&    
    ( exists c:int::     
      (( packed[this,countP] &&
@@ -156,8 +145,7 @@ ensures ( packed[this, parentP] ==>
            ( packed[parent[this], rightP] && (rcRightPred[parent[this]]==c)  && (frac[parent[this], rightP] >= 50))
            ) ) )
      &&
-     ((parent[this]==null) ==> packed[this,countP] && (cCountPred[this] == c) && (frac[this,countP]>=50) )  ) ))
-  )  );
+     ((parent[this]==null) ==> packed[this,countP] && (cCountPred[this] == c) && (frac[this,countP]>=50) )  ) ));
 
 
 //axioms about the existance of a variable 
@@ -176,6 +164,26 @@ axiom (forall this: Ref, left: [Ref]Ref, right: [Ref]Ref,  cCountPred : [Ref]int
     (exists c:int :: packed[this, countP] && (cCountPred[this] == c)  ==> ( packed[this, countP] && (cCountPred[this] == count[this]) ) )
 );
 
+function countPredFunc(this: Ref, count: [Ref]int,  lc1:int, rc1:int, 
+        lcLeftPred : [Ref]int, rcRightPred : [Ref]int, packed: PackedType, frac: FractionType) : bool;
+
+//axiom about existance of variable, but the other way of the implication
+axiom (forall this: Ref, left: [Ref]Ref, right: [Ref]Ref, count: [Ref]int,  lc1:int, rc1:int, 
+        lcLeftPred : [Ref]int, rcRightPred : [Ref]int, packed: PackedType, frac: FractionType::
+    (
+(
+  ( packed[this, leftP] && (lcLeftPred[this] == lc1) && 
+  (frac[this, leftP] >= 50) &&
+  packed[this, rightP] &&
+  (rcRightPred[this] == rc1) &&
+(frac[this, rightP] >= 50) && 
+ (count[this] == lc1+rc1+1) )
+)
+ ==> countPredFunc(this, count,  lc1, rc1, 
+        lcLeftPred, rcRightPred, packed, frac)
+) 
+);
+
 
 procedure Composite(this:Ref)
 modifies left, right, parent, count, frac, packed;
@@ -184,142 +192,32 @@ ensures packed[this, parentP];
 ensures packed[this, leftP] && (lcLeftPred[this] == 0);
 ensures packed[this, rightP] && (rcRightPred[this] == 0);
 ensures (frac[this, parentP] >= 50) && (frac[this, leftP] >= 50) && (frac[this, rightP] >= 50) ;
-ensures packed[this, parentP];
 {
+
   count[this] := 1;
   left[this] := null;
   right[this] := null;
   parent[this] := null;
+call PackLeftNull(this, 0);
+packed[this, leftP] := true;
+frac[this, leftP] := 100;
+call PackRightNull(this,0);
+packed[this, rightP] := true;
+frac[this, rightP] :=100;
 
-  frac[this, leftP] := 100;
+//need to put in the assertions that are related to exists
+//Boogie does not know how to intantiate the exists but we know
+assert countPredFunc(this, count,  0, 0, 
+        lcLeftPred, rcRightPred, packed, frac);
 
-  frac[this, rightP] :=100;
-
-  frac[this, countP] := 100;
-
-  frac[this, parentP] := 100;
-  packed[this, parentP]:=true;
+call PackCount(this,1);
+packed[this, countP] := true;
+ frac[this, countP] := 100;
+call PackParentNull(this);
+packed[this, parentP] := true;
+frac[this, parentP] := 100;
 }
 
-procedure updateCountRec(this: Ref)
-modifies count, frac, packed;
-requires this!=null;
-requires packed[this, parentP] == false;
-requires parent[this]!=null ==> (frac[parent[this], parentP]>0);
-requires (parent[this]!=null) && (this==right[parent[this]]) ==> (frac[parent[this], rightP]>=50);
-requires (parent[this]!=null) && (this==left[parent[this]]) ==> (frac[parent[this], leftP]>=50);
-requires parent[this]==null ==> (frac[this, countP] >= 50);
-requires (forall r:Ref:: (r!=this) ==> packed[r, countP]);
-requires packed[this, leftP];
-requires packed[this, rightP];
-requires (frac[this,leftP] >=50) &&   (frac[this,rightP] >=50);
-requires (frac[this, countP] >= 50);
-
-ensures   (packed[this, parentP]);    
-
-{
- var fracLocal: FractionType;
-
-  if (parent[this] != null)
- {
-
-//we assert what is true when packed[this, parentP]==false
-assert frac[this, countP]>=50;
-fracLocal[this, countP]:=frac[this, countP];
-
-//this asserts that we have a fraction to parentP
-assert (frac[parent[this], parentP]>0);
-//we unpack parent[this] from parentP
-//might need to say that other objects are not unpacked for parentP
-packed[parent[this], parentP]:=false;
-assert (forall r:Ref:: (r!=this) ==> (packed[r, countP]));
-
-//we can assume this because we just unpacked
-//parent[this] from parentP
-assume frac[parent[this], countP]>=50;
-fracLocal[parent[this], countP]:=frac[parent[this], countP];
-
-
-//we unpack parent[this] from countP
-packed[parent[this], countP]:=false;
-
-//we can assume this because we just unpacked parent[this] from countP
-assume (frac[this,leftP]>=50) && (frac[this,rightP]>=50);
-fracLocal[parent[this], rightP]:=frac[parent[this], rightP];
-
-
-//we assume this is the right child of parent[this]
-//the other case is analogous
-assume this==right[parent[this]];
-assert (parent[this]!=null) && (this==right[parent[this]]) ==> frac[parent[this],rightP]>=50;
-fracLocal[parent[this],rightP]:=fracLocal[parent[this], rightP] +frac[parent[this],rightP];
-
-assert (fracLocal[parent[this],rightP]>=100);
-//unpack parent[this] from rightP
-packed[parent[this], rightP]:=false;
-assert  (packed[parent[this],rightP]==false)  ==> frac[right[parent[this]],countP]>=50;
-fracLocal[this, countP]:=fracLocal[this, countP]+frac[this, countP];
-
-assert (frac[this,leftP] >=50) &&   (frac[this,rightP] >=50);
-assert packed[this, parentP]==false;
-frac[this, countP]:=fracLocal[this, countP];
-assert (frac[this, countP] >= 100);
-assert packed[this, rightP] && (rcRightPred[this] == count[right[this]]);
-assert (exists c2:int :: packed[this, rightP] && (rcRightPred[this] == c2));
-packed[this, rightP]:=true;
-assert packed[this, leftP] && (lcLeftPred[this] == count[left[this]]);
-assert (exists c1:int :: packed[this, leftP] && (lcLeftPred[this] == c1)); 
-packed[this, leftP]:=true;
-      call updateCount(this);
-assert (exists c:int ::
-          packed[this, countP] && (cCountPred[this] == c)
-         );
-assert packed[this, countP] && (cCountPred[this] == count[this]);
-assert packed[this, countP];
-assert (frac[this, countP]>=100)  ; 
-
-//assert the preconditions of updateCountRec
-assert parent[this]!=null;
-packed[parent[this], parentP]:=false;
-
-//we can assume these because we have just unpacked parent[this] from parentP
-assume parent[parent[this]]!=null ==> ( frac[parent[parent[this]], parentP]>0);
-assume parent[parent[this]]==null ==> (frac[parent[this], countP] >= 50);
-assume (parent[parent[this]]!=null) && (this==right[parent[parent[this]]]) ==> (frac[parent[parent[this]], rightP]>=50);
-assume (parent[parent[this]]!=null) && (this==left[parent[parent[this]]]) ==> (frac[parent[parent[this]], leftP]>=50);
-
-
-assert packed[parent[this], rightP] && (rcRightPred[parent[this]] == count[this]);
-assert (exists c2:int :: packed[parent[this], rightP] && (rcRightPred[parent[this]] == c2));
-packed[parent[this],rightP]:=true;
-assert (forall r:Ref:: (r!=parent[this]) ==> (packed[r, countP]));
-
-//assertions for proving isPackedLeftPred(parent[this]...
-//we assume this, the other case is trivial
-//we could write a new procedure for the other case?
-assume left[parent[this]] != null;
-assert packed[left[parent[this]], countP];
-//we can assume this because isPackedCountPred is packed for left[parent[this]]
-assume packed[left[parent[this]], countP] && (cCountPred[left[parent[this]]]==count[this]);
-
-assert packed[parent[this], leftP] && (lcLeftPred[parent[this]]== count[left[parent[this]]]);
-assert (exists c1:int :: packed[parent[this], leftP] && (lcLeftPred[parent[this]]== c1)); 
-packed[parent[this],leftP]:=true;
-      call updateCountRec(parent[this]);
-      }
-    else
-  { 
-assert (frac[this, countP] >= 50);
-fracLocal[this, countP]:=frac[this, countP];
-assert  parent[this]==null ==> (frac[this, countP] >= 50);
-fracLocal[this, countP]:=fracLocal[this, countP] + frac[this, countP];
-frac[this, countP]:=fracLocal[this, countP];
-assert (frac[this, countP] >= 100);    
- 
-         call updateCount(this);
-
-  }  
- }
 
 
  
@@ -330,11 +228,9 @@ assert (frac[this, countP] >= 100);
  requires packed[this, rightP];
  requires (frac[this,leftP] >=50) &&   (frac[this,rightP] >=50)  && (frac[this, countP] >= 100);
         
-ensures ( exists c:int :: packed[this, countP] && (cCountPred[this]==c)
-         );
+ensures ( exists c:int :: (cCountPred[this]==c));
 ensures packed[this, countP];
 ensures (frac[this, countP]>=100);
-ensures (forall r:Ref:: (r!=this) ==> (packed[r, countP]==old(packed[r, countP])));
      
 
  {
@@ -344,12 +240,22 @@ ensures (forall r:Ref:: (r!=this) ==> (packed[r, countP]==old(packed[r, countP])
 
         if (left[this] != null)
            {
-       newc := newc + count[left[this]];
+ 	call UnpackLeftNotNull(this, lcLeftPred[this]);
+	packed[this, leftP]:=false;
+	call UnpackCount(left[this], cCountPred[left[this]]);
+	packed[left[this], countP]:=false; 
+        newc := newc + count[left[this]];
+	assert countPredFunc(left[this], count,  lcLeftPred[left[this]],  rcRightPred[left[this]], 
+        lcLeftPred, rcRightPred, packed, frac);
+	call PackCount(left[this], cCountPred[left[this]]);
+	packed[left[this], countP]:=true;
        }
        
         if (right[this] != null)
              {
-         
+         call UnpackRightNotNull(this, rcRightPred[this]);
+	 packed[this, rightP]:=false;
+	call UnpackCount(right[this], cCountPred[right[this]]);
          newc := newc + count[right[this]];
          
        }
@@ -359,34 +265,4 @@ ensures (forall r:Ref:: (r!=this) ==> (packed[r, countP]==old(packed[r, countP])
  
     packed[this, countP]:=true;
     
-      }
-
-
-procedure setLeft(this: Ref, l:Ref)
-modifies parent, left, count, frac, packed;
-requires this!=null;
-requires this!=l;
-requires l!=null;
-requires packed[this, parentP];
-requires packed[l, parentP];
-requires (forall r:Ref:: packed[r, countP]);
-ensures packed[this, parentP];
- {
-
-packed[this, parentP]:=false;
-
-
-   parent[l]:=this;
-   left[this]:=l;
-
-
-packed[this, leftP]:=true;
-
-packed[this, rightP]:=true;
-
-packed[this, countP]:=false;
-
-
-   call updateCountRec(this);
-   
 }
