cells1.bpl
@@ -289,12 +289,3 @@ call setInputDep(this, out[this]);
 assume xIn2Pred[this] == x;
 call PackOK(this);
 }
-
-
- 
-
-
-
-
-
-
