doubleCount1.bpl
@@ -3,33 +3,33 @@ type Ref;
 type PredicateTypes;
 type FractionType = [Ref, PredicateTypes] int;
 type PackedType = [Ref, PredicateTypes] bool;
-
+var packed: PackedType;
+var frac: FractionType;
 const null: Ref;
-const unique okP: PredicateTypes;
 
 var val: [Ref]int;
 var dbl: [Ref]int;
-var packed: PackedType;
-var frac: FractionType;
+
+const unique okP: PredicateTypes;
 
 procedure PackOK(this:Ref);
-ensures (dbl[this]==val[this]*2) ==> packed[this, okP];
+requires (dbl[this]==val[this]*2);
 
 procedure UnpackOK(this:Ref);
-ensures packed[this, okP] ==> (dbl[this]==val[this]*2);
+requires packed[this, okP];
+ensures (dbl[this]==val[this]*2);
 
 
 procedure increment(this: Ref)
-modifies val, dbl, packed;
-requires packed[this, okP];
-requires frac[this, okP] >0;
-ensures  packed[this, okP];
-ensures frac[this, okP] >0;
+modifies val, dbl, packed, frac;
+requires packed[this, okP]  && (frac[this, okP] > 0);
+ensures  packed[this, okP] && (frac[this, okP] > 0);
 {
 call UnpackOK(this);
 packed[this, okP]:=false;
 val[this]:= val[this]+1;
-dbl[this]:=dbl[this]+2;
+dbl[this]:= dbl[this]+2;
 call PackOK(this);
+packed[this, okP]:=true;
 }
 
